change SimMemInjInv

demo/mutrec/SimMemInjInv.v
@@ -14,6 +14,7 @@ Require Import Conventions1.
 Require MachC.
 Require Export SimMemInj.
 Require Import SimMemInjC.
+Require Import Coq.Logic.FunctionalExtensionality.
 
 Set Implicit Arguments.
 
@@ -21,91 +22,84 @@ Set Implicit Arguments.
 
 Section MEMINJINV.
 
-  Variable P : memory_chunk -> Z -> option val -> Prop.
+  Definition memblk_invariant := (memory_chunk -> Z -> option val) -> Prop.
+  (* Definition memory_invariant := block -> memblk_invariant -> Prop. *)
 
-  Record t' := mk
-    { minj:> SimMemInj.t';
-      src_genv_nb : block;
-      tgt_genv_nb : block;
-      mem_inv: block -> Prop;
-      (* mem_inv: block -> (memory_chunk -> Z -> option val -> Prop); *)
-    }.
+  Variable P : memblk_invariant.
 
-  (* Record t' := *)
-  (*   mk *)
-  (*     { src : mem; *)
-  (*       tgt : mem; *)
-  (*       inj : meminj; *)
-  (*       mem_inv: block -> option (memory_chunk -> Z -> val -> Prop); *)
-  (*     }. *)
+  (* Record t' := mk *)
+  (*   { minj:> SimMemInj.t'; *)
+  (*     src_genv_nb : block; *)
+  (*     tgt_genv_nb : block; *)
+  (*     mem_inv: block -> Prop; *)
+  (*     (* mem_inv: block -> (memory_chunk -> Z -> option val -> Prop); *) *)
+  (*   }. *)
 
-  Definition tgt_private_nge (sm: t') :=
-    (loc_out_of_reach sm.(inj) sm.(src))
-      /2\ (valid_blocks sm.(tgt)) /2\ (fun blk _ => Ple blk sm.(tgt_genv_nb)).
+  Record t' :=
+    mk
+      { src : mem;
+        tgt : mem;
+        inj : meminj;
+        mem_inv: block -> Prop;
+        (* mem_inv: memory_invariant; *)
+      }.
 
-  Definition src_private_nge (sm: t') :=
-    (loc_unmapped sm.(inj))
-      /2\ (valid_blocks sm.(src)) /2\ (fun blk _ => Ple blk sm.(src_genv_nb)).
+  (* Definition tgt_private_nge (sm: t') := *)
+  (*   (loc_out_of_reach sm.(inj) sm.(src)) *)
+  (*     /2\ (valid_blocks sm.(tgt)) /2\ (fun blk _ => Ple blk sm.(tgt_genv_nb)). *)
 
-  Inductive invariant_satisfied (invar : block -> Prop) (m: mem): Prop :=
-  | invariant_satisfied_intro
-      (SAT: forall
-          blk chunk ofs v
-          (INV: invar blk)
-          (LOAD: Mem.load chunk m blk ofs = v),
-          P chunk ofs v)
-      (WRITABLE: forall
-          blk chunk ofs
-          (INV: invar blk),
-          Mem.valid_access m chunk blk ofs Writable).
+  (* Definition src_private_nge (sm: t') := *)
+  (*   (loc_unmapped sm.(inj)) *)
+  (*     /2\ (valid_blocks sm.(src)) /2\ (fun blk _ => Ple blk sm.(src_genv_nb)). *)
+
+  Definition inv_sat_blk blk (invar: memblk_invariant) (m: mem): Prop :=
+    invar (fun chunk ofs =>
+             if (Mem.valid_access_dec m chunk blk ofs Writable)
+             then Mem.load chunk m blk ofs
+             else None).
+
+  (* Definition inv_sat_mem (invar: memory_invariant) (m: mem) : Prop := *)
+  (*   forall blk inv_blk (INVAR: invar blk inv_blk), inv_sat_blk blk inv_blk m.   *)
+
+  Definition inv_sat_mem (invar: block -> Prop) (m: mem) : Prop :=
+    forall blk (INVAR: invar blk), inv_sat_blk blk P m.
 
   Inductive wf' (sm0: t'): Prop :=
   | wf_intro
-      (WF: SimMemInj.wf' sm0)
-      (SAT: invariant_satisfied sm0.(mem_inv) sm0.(SimMemInj.tgt))
+      (WF: Mem.inject sm0.(inj) sm0.(src) sm0.(tgt))
+      (SAT: inv_sat_mem sm0.(mem_inv) sm0.(tgt))
       (INVRANGE: forall blk ofs (INV: sm0.(mem_inv) blk),
-          tgt_private sm0 blk ofs /\ Plt blk sm0.(tgt_genv_nb))
-      (SRCGENB: Ple sm0.(src_genv_nb) sm0.(src_parent_nb))
-      (TGTGENB: Ple sm0.(tgt_genv_nb) sm0.(tgt_parent_nb))
-      (SRCEXTGE: forall blk ofs (EXTERN: src_external sm0 blk ofs),
-          Ple sm0.(src_genv_nb) blk)
-      (TGTEXTGE: forall blk ofs (EXTERN: tgt_external sm0 blk ofs),
-          Ple sm0.(tgt_genv_nb) blk)
+          loc_out_of_reach sm0.(inj) sm0.(src) blk ofs /\ Mem.valid_block sm0.(tgt) blk)
+      (* (INVRANGE: forall blk ofs invar (INV: sm0.(mem_inv) blk invar),         *)
+      (*     loc_out_of_reach sm0.(inj) sm0.(src) blk ofs /\ Mem.valid_block sm0.(tgt) blk) *)
   .
 
   Lemma unchanged_on_invariant invar m0 m1
-        (INVAR: invariant_satisfied invar m0)
+        (INVAR: inv_sat_mem invar m0)
         (INVRANGE: invar <1= Mem.valid_block m0)
         (UNCH: Mem.unchanged_on (fun blk _ => invar blk) m0 m1)
     :
-      invariant_satisfied invar m1.
+      inv_sat_mem invar m1.
   Proof.
-    inv INVAR. econs.
-    - i. eapply SAT; eauto.
-      erewrite <- Mem.load_unchanged_on_1; eauto.
-    - i. unfold Mem.valid_access in *.
-      exploit WRITABLE; eauto. i. des.
-      split; eauto. ii.
-      eapply Mem.perm_unchanged_on; eauto.
+    ii. exploit INVAR; eauto. intros SAT.
+    unfold inv_sat_blk in *. rp; eauto.
+    extensionality chunk. extensionality ofs.
+    des_ifs.
+    - eapply Mem.load_unchanged_on_1; eauto.
+    - exfalso. apply n. inv v. split; auto.
+      ii. eapply Mem.perm_unchanged_on_2; eauto.
+    - exfalso. apply n. inv v. split; auto.
+      ii. eapply Mem.perm_unchanged_on; eauto.
   Qed.
-
-  Definition lift' (mrel0: t'): t' :=
-    mk (SimMemInj.mk mrel0.(src) mrel0.(tgt) mrel0.(inj) mrel0.(src_private_nge) mrel0.(tgt_private_nge) mrel0.(src_parent_nb) mrel0.(tgt_parent_nb))
-       (mrel0.(src_parent_nb))
-       (mrel0.(tgt_parent_nb))
-       (mrel0.(mem_inv)).
-
-  Definition unlift' (mrel0 mrel1: t'): t' :=
-    mk (SimMemInj.mk mrel1.(src) mrel1.(tgt) mrel1.(inj) mrel0.(src_external) mrel0.(tgt_external) mrel0.(src_parent_nb) mrel0.(tgt_parent_nb))
-       (mrel0.(src_parent_nb))
-       (mrel0.(tgt_parent_nb))
-       (mrel0.(mem_inv)).
 
   Inductive le' (mrel0 mrel1: t'): Prop :=
   | le_intro
-      (MLE: SimMemInj.le' mrel0 mrel1)
-      (SRCGENBEQ: mrel0.(src_genv_nb) = mrel1.(src_genv_nb))
-      (TGTGENBEQ: mrel0.(tgt_genv_nb) = mrel1.(tgt_genv_nb))
+      (SRCNBLE: Ple mrel0.(src).(Mem.nextblock) mrel1.(src).(Mem.nextblock))
+      (TGTNBLE: Ple mrel0.(tgt).(Mem.nextblock) mrel1.(tgt).(Mem.nextblock))
+      (INCR: inject_incr mrel0.(inj) mrel1.(inj))
+      (FROZEN: inject_separated
+               (mrel0.(inj)) (mrel1.(inj))
+               (mrel0.(src)) (mrel0.(tgt)))
       (MINVEQ: mrel0.(mem_inv) = mrel1.(mem_inv))
   .
 
@@ -117,30 +111,38 @@ Section MEMINJINV.
       tgt := tgt;
       wf := wf';
       le := le';
-      lift := lift';
-      unlift := unlift';
+      lift := fun sm => sm;
+      unlift := fun _ sm => sm;
       sim_val := fun (mrel: t') => Val.inject mrel.(inj);
       sim_val_list := fun (mrel: t') => Val.inject_list mrel.(inj);
     }.
   Next Obligation.
     econs.
-    - econs; ss. refl.
-    - ii. inv H. inv H0. econs; etrans; eauto.
+    - econs; ss.
+      + refl.
+      + refl.
+      + ii. clarify.
+    - ii. inv H. inv H0. econs; eauto.
+      + etrans; eauto.
+      + etrans; eauto.
+      + etrans; eauto.
+      + ii. destruct (inj y b1) as [[b3 delta0]|] eqn:DELTA.
+        * dup DELTA. eapply INCR0 in DELTA. clarify.
+          exploit FROZEN; eauto.
+        * dup DELTA. exploit FROZEN0; eauto. i. des.
+          unfold Mem.valid_block in *. split; ii.
+          { eapply H1. eapply Plt_Ple_trans; eauto. }
+          { eapply H2. eapply Plt_Ple_trans; eauto. }
+      + etrans; eauto.
   Qed.
   Next Obligation.
-    admit "ez - find this lemma".
+    inv MLE. ii. eapply val_inject_incr; eauto.
   Qed.
   Next Obligation.
-    admit "ez - find this lemma".
-  Qed.
-  Next Obligation.
-    admit "ez - find this lemma".
-  Qed.
-  Next Obligation.
-    admit "ez - find this lemma".
-  Qed.
-  Next Obligation.
-    admit "ez - find this lemma".
+    extensionality l0. extensionality l1. eapply prop_ext2.
+    induction x0; ss; i; split; intros H; inv H; econs; eauto.
+    - eapply IHx0; eauto.
+    - eapply IHx0; eauto.
   Qed.
 
   Lemma mem_inv_le sm0 sm1
@@ -151,177 +153,217 @@ Section MEMINJINV.
     inv MLE. rewrite MINVEQ. auto.
   Qed.
 
-  Definition update (sm0: t') (src tgt: mem) (inj: meminj) :=
-    mk (SimMemInjC.update sm0 src tgt inj) (sm0.(src_genv_nb)) (sm0.(tgt_genv_nb)) (sm0.(mem_inv)).
-
 End MEMINJINV.
 
 
 Section SIMSYMBINV.
 
-Variable P : memory_chunk -> Z -> option val -> Prop.
+  Variable P : memblk_invariant.
 
-Inductive le (ss0: ident -> Prop) (sk_src sk_tgt: Sk.t) (ss1: ident -> Prop): Prop :=
-| symb_le_intro
-    (LE: ss0 <1= ss1)
-    (OUTSIDE: forall
-        id
-        (IN: (ss1 -1 ss0) id)
-      ,
-        <<OUTSIDESRC: ~ sk_src.(defs) id>> /\ <<OUTSIDETGT: ~ sk_tgt.(defs) id>>)
-.
+  Inductive le (ss0: ident -> Prop) (sk_src sk_tgt: Sk.t) (ss1: ident -> Prop): Prop :=
+  | symb_le_intro
+      (LE: ss0 <1= ss1)
+      (OUTSIDE: forall
+          id
+          (IN: (ss1 -1 ss0) id)
+        ,
+          <<OUTSIDESRC: ~ sk_src.(defs) id>> /\ <<OUTSIDETGT: ~ sk_tgt.(defs) id>>)
+  .
 
-Inductive skenv_inject {F V} (ge: Genv.t F V) (j: meminj)
-          (invar: block -> Prop) : Prop :=
-| sken_inject_intro
-    (DOMAIN: forall b, Plt b ge.(Genv.genv_next) ->
-                       forall (NINV: ~ invar b), j b = Some(b, 0))
-    (NDOMAIN: forall b, Plt b ge.(Genv.genv_next) ->
-                       forall (NINV: invar b), j b = None)
-    (IMAGE: forall b1 b2 delta, j b1 = Some(b2, delta) -> Plt b2 ge.(Genv.genv_next) -> b1 = b2)
-.
+  Inductive skenv_inject {F V} (ge: Genv.t F V) (j: meminj)
+            (invar: block -> Prop) : Prop :=
+  | sken_inject_intro
+      (DOMAIN: forall b, Plt b ge.(Genv.genv_next) ->
+                         forall (NINV: ~ invar b), j b = Some(b, 0))
+      (NDOMAIN: forall b, Plt b ge.(Genv.genv_next) ->
+                          forall (NINV: invar b), j b = None)
+      (IMAGE: forall b1 b2 delta, j b1 = Some(b2, delta) -> Plt b2 ge.(Genv.genv_next) -> b1 = b2)
+  .
 
-Inductive invariant_globvar F V: globdef F V -> Prop :=
-| invariant_globvar_intro
-    v
-    (INITD: admit "about init data" v.(gvar_init))
-  :
-    invariant_globvar (Gvar v)
-.
+  Inductive invariant_globvar F V: globdef F V -> Prop :=
+  | invariant_globvar_intro
+      v
+      (INITD: admit "about init data" v.(gvar_init))
+    :
+      invariant_globvar (Gvar v)
+  .
 
-Inductive sim_skenv_inj (sm: t') (ss: ident -> Prop) (skenv_src skenv_tgt: SkEnv.t): Prop :=
-| sim_skenv_inj_intro
-    (INVCOMPAT: forall id blk (FIND: skenv_tgt.(Genv.find_symbol) id = Some blk),
-        ss id <-> sm.(mem_inv) blk)
-    (PUBKEPT: (fun id => In id skenv_src.(Genv.genv_public)) <1= ~1 ss)
-    (INJECT: skenv_inject skenv_src sm.(inj) sm.(mem_inv))
-    (BOUNDSRC: Ple skenv_src.(Genv.genv_next) sm.(src_parent_nb))
-    (BOUNDTGT: Ple skenv_src.(Genv.genv_next) sm.(tgt_parent_nb))
-    (SIMSKENV: SimSymbId.sim_skenv skenv_src skenv_tgt)
-    (SRCGENB: Genv.genv_next skenv_src = sm.(src_genv_nb))
-    (TGTGENB: Genv.genv_next skenv_tgt = sm.(tgt_genv_nb))
-.
+  Inductive sim_skenv_inj (sm: t') (ss: ident -> Prop) (skenv_src skenv_tgt: SkEnv.t): Prop :=
+  | sim_skenv_inj_intro
+      (INVCOMPAT: forall id blk (FIND: skenv_tgt.(Genv.find_symbol) id = Some blk),
+          ss id <-> sm.(mem_inv) blk)
+      (PUBKEPT: (fun id => In id skenv_src.(Genv.genv_public)) <1= ~1 ss)
+      (INJECT: skenv_inject skenv_src sm.(inj) sm.(mem_inv))
+      (BOUNDSRC: Ple skenv_src.(Genv.genv_next) sm.(src).(Mem.nextblock))
+      (BOUNDTGT: Ple skenv_src.(Genv.genv_next) sm.(tgt).(Mem.nextblock))
+      (SIMSKENV: SimSymbId.sim_skenv skenv_src skenv_tgt)
+  .
 
-Inductive sim_sk (ss: ident -> Prop) (sk_src sk_tgt: Sk.t): Prop :=
-| sim_sk_intro
-    (SKSAME: sk_src = sk_tgt)
-    (CLOSED: forall id (SS: ss id),
-        exists g,
-          (<<DEF: sk_tgt.(prog_defmap) ! id = Some g>>) /\
-          (<<INV: invariant_globvar g>>) /\
-          (<<PRVT: ~ In id (prog_public sk_tgt)>>)).
+  Inductive sim_sk (ss: ident -> Prop) (sk_src sk_tgt: Sk.t): Prop :=
+  | sim_sk_intro
+      (SKSAME: sk_src = sk_tgt)
+      (CLOSED: forall id (SS: ss id),
+          exists g,
+            (<<DEF: sk_tgt.(prog_defmap) ! id = Some g>>) /\
+            (<<INV: invariant_globvar g>>) /\
+            (<<PRVT: ~ In id (prog_public sk_tgt)>>)).
 
-Global Program Instance SimSymbIdInv: SimSymb.class (SimMemInjInv P) := {
-  t := ident -> Prop;
-  le := le;
-  sim_sk := sim_sk;
-  sim_skenv := sim_skenv_inj;
-}
-.
-Next Obligation.
-  econs; eauto. i. des. clarify.
-Qed.
-Next Obligation.
-  admit "ez - copy SimSymbDrop".
-Qed.
-Next Obligation.
-  inv SIMSK. eauto.
-Qed.
-Next Obligation.
-  inv SIMSK. inv SIMSK0. exists (ss0 \1/ ss1).
-  admit "copy SimSymbDrop".
-Qed.
-Next Obligation.
-  inv SIMSKE. inv SIMSKENV. eauto.
-Qed.
-Next Obligation.
-  inv SIMSK. eexists.
-  assert (SS: forall id, {ss id} + {~ ss id}).
-  { admit "choice + classic". }
-  set (j := fun blk => if (plt blk (Mem.nextblock m_src))
-                       then match Genv.invert_symbol (Sk.load_skenv sk_tgt) blk with
-                            | Some id =>
-                              if (SS id) then None else Some (blk, 0)
-                            | None => None
-                            end
-                       else None).
-  eexists (mk (SimMemInj.mk _ _ j bot2 bot2 _ _) _ _ _). ss.
-  instantiate (1:=fun blk => exists id,
-                      (<<FIND: (Sk.load_skenv sk_tgt).(Genv.find_symbol) id = Some blk>>) /\
-                      (<<SINV: ss id>>)).
-  esplits; eauto.
-  - econs; ss; eauto.
-    + i. split; i; eauto. des.
-      apply Genv.find_invert_symbol in FIND.
-      apply Genv.find_invert_symbol in H. clarify.
-    + ii. exploit CLOSED; eauto. i. des.
-      apply PRVT. rewrite <- Genv.globalenv_public. auto.
-    + admit "".
-    + refl.
-    + refl.
-  - econs; ss; eauto.
-    + econs; ss; eauto.
-      * admit "".
-      * unfold Sk.load_mem in *.
+  Global Program Instance SimSymbIdInv: SimSymb.class (SimMemInjInv P) :=
+    {
+      t := ident -> Prop;
+      le := le;
+      sim_sk := sim_sk;
+      sim_skenv := sim_skenv_inj;
+    }
+  .
+  Next Obligation.
+    econs; eauto. i. des. clarify.
+  Qed.
+  Next Obligation.
+    admit "ez - copy SimSymbDrop".
+  Qed.
+  Next Obligation.
+    inv SIMSK. eauto.
+  Qed.
+  Next Obligation.
+    inv SIMSK. inv SIMSK0. exists (ss0 \1/ ss1).
+    admit "copy SimSymbDrop".
+  Qed.
+  Next Obligation.
+    inv SIMSKE. inv SIMSKENV. eauto.
+  Qed.
+  Next Obligation.
+    inv SIMSK. eexists.
+    assert (SS: forall id, {ss id} + {~ ss id}).
+    { admit "choice + classic". }
+    set (j := fun blk => if (plt blk (Mem.nextblock m_src))
+                         then match Genv.invert_symbol (Sk.load_skenv sk_tgt) blk with
+                              | Some id =>
+                                if (SS id) then None else Some (blk, 0)
+                              | None => None
+                              end
+                         else None).
+    eexists (mk _ _ j _). ss.
+    instantiate (1:=fun blk => exists id,
+                        (<<FIND: (Sk.load_skenv sk_tgt).(Genv.find_symbol) id = Some blk>>) /\
+                        (<<SINV: ss id>>)).
+    esplits; eauto.
+    - econs; ss; eauto.
+      + i. split; i; eauto. des.
+        apply Genv.find_invert_symbol in FIND.
+        apply Genv.find_invert_symbol in H. clarify.
+      + ii. exploit CLOSED; eauto. i. des.
+        apply PRVT. rewrite <- Genv.globalenv_public. auto.
+      + admit "".
+      + unfold Sk.load_mem in *.
         apply Genv.init_mem_genv_next in LOADMEMSRC.
         rewrite <- LOADMEMSRC. refl.
-      * unfold Sk.load_mem in *.
+      + unfold Sk.load_mem in *.
         apply Genv.init_mem_genv_next in LOADMEMSRC.
         rewrite <- LOADMEMSRC. refl.
-    + admit "fill invariant_globvar".
-    + i. unfold tgt_private. ss. des. splits; auto.
-      * ii. unfold j in *. des_ifs.
-        apply Genv.find_invert_symbol in INV. clarify.
-      * unfold Sk.load_mem, Sk.load_skenv in *.
-        eapply Genv.find_symbol_not_fresh; eauto.
-      * eapply Genv.genv_symb_range; eauto.
-    + refl.
-    + refl.
-Qed.
-Next Obligation.
-  destruct sm0, sm1. inv MLE. inv MLE0. ss. clarify.
-  inv SIMSKENV. econs; ss; eauto.
-  - inv INJECT. econs; eauto.
-    + i. destruct (inj minj1 b) eqn:BLK; auto. destruct p. exfalso.
-      inv FROZEN. exploit NEW_IMPLIES_OUTSIDE; eauto.
-      i. des. eapply Plt_strict. eapply Plt_Ple_trans.
-      * apply H.
-      * transitivity (src_parent_nb minj0); eauto.
-    + i. destruct (inj minj0 b1) eqn:BLK.
-      * destruct p. dup BLK. apply INCR in BLK. clarify.
-        eapply IMAGE; eauto.
-      * inv FROZEN. exploit NEW_IMPLIES_OUTSIDE; eauto.
-        i. des. exfalso. eapply Plt_strict. eapply Plt_Ple_trans.
-        { apply H0. }
-        { etrans; eauto. }
-  - rewrite <- SRCPARENTEQNB. auto.
-  - rewrite <- TGTPARENTEQNB. auto.
-Qed.
-Next Obligation.
-Admitted.
-Next Obligation.
-Admitted.
-Next Obligation.
-Admitted.
-Next Obligation.
-Admitted.
-Next Obligation.
-  inv SIMSKENV. inv SIMSKENV0.
-  inv ARGS. ss.
-  exploit ec_mem_inject; eauto.
-  - eapply external_call_spec.
-  - instantiate (1:=skenv_sys_tgt).
-    admit "ez".
-  - instantiate (1:=tgt sm0). rewrite MEMSRC.
-    inv MWF. inv WF. eauto.
-  - i. des.
-    eexists (mk (SimMemInj.mk (Retv.m retv_src) m2' f' _ _ _ _) _ _ _). ss.
-    exists (Retv.mk vres' m2'). ss.
-    esplits; ss; eauto.
-    + rewrite MEMTGT. eauto.
-    + admit "".
-    + admit "".
-      Unshelve. all:admit"".
-Qed.
+
+    - econs; ss; eauto.
+      + admit "copy SimSymbId".
+        (* econs; ss; eauto. *)
+        (* * *)
+        (*   econs; eauto; ii; unfold j in *; des_ifs; clarify. *)
+        (*   { zsimpl. auto. } *)
+        (*   { apply Z.divide_0_r. } *)
+        (*   { zsimpl. admit "TODO". } *)
+        (* * ii. unfold j. des_ifs. *)
+        (* * ii. unfold j in *. des_ifs. *)
+        (* * ii. unfold j in *. des_ifs. auto. *)
+        (* * ii. unfold j in *. des_ifs. *)
+        (*   admit "TODO". *)
+      + admit "fill invariant_globvar".
+      + i. split.
+        * unfold j. ii. des_ifs.
+          des. eapply Genv.find_invert_symbol in INV. clarify.
+        * des. eapply Genv.genv_symb_range in INV.
+          unfold Sk.load_skenv, Sk.load_mem in *. ss.
+          apply Genv.init_mem_genv_next in LOADMEMSRC.
+          rewrite LOADMEMSRC in *. auto.
+  Qed.
+  Next Obligation.
+  Admitted.
+  (*   destruct sm0, sm1. inv MLE. ss. clarify. *)
+  (*   inv SIMSKENV. econs; ss; eauto. *)
+  (*   - inv INJECT. econs; eauto. *)
+  (*     + i. destruct (inj minj1 b) eqn:BLK; auto. destruct p. exfalso. *)
+  (*       inv FROZEN. exploit NEW_IMPLIES_OUTSIDE; eauto. *)
+  (*       i. des. eapply Plt_strict. eapply Plt_Ple_trans. *)
+  (*       * apply H. *)
+  (*       * transitivity (src_parent_nb minj0); eauto. *)
+  (*     + i. destruct (inj minj0 b1) eqn:BLK. *)
+  (*       * destruct p. dup BLK. apply INCR in BLK. clarify. *)
+  (*         eapply IMAGE; eauto. *)
+  (*       * inv FROZEN. exploit NEW_IMPLIES_OUTSIDE; eauto. *)
+  (*         i. des. exfalso. eapply Plt_strict. eapply Plt_Ple_trans. *)
+  (*         { apply H0. } *)
+  (*         { etrans; eauto. } *)
+  (*   - rewrite <- SRCPARENTEQNB. auto. *)
+  (*   - rewrite <- TGTPARENTEQNB. auto. *)
+  (* Qed. *)
+  Next Obligation.
+  Admitted.
+  Next Obligation.
+  Admitted.
+  Next Obligation.
+  Admitted.
+  Next Obligation.
+    inv SIMSKENV. inv SIMSKENV0.
+    inv ARGS. inv MWF. ss.
+    exploit ec_mem_inject; eauto.
+    - eapply external_call_spec.
+    - instantiate (1:=skenv_sys_tgt).
+      inv INJECT. econs; ss. splits.
+      + i. destruct (classic (mem_inv sm0 b1)).
+        { exfalso. eapply NDOMAIN in H1.
+          - clarify.
+          - eapply Genv.genv_symb_range; eauto. }
+        exploit DOMAIN; eauto.
+        { eapply Genv.genv_symb_range; eauto. }
+        i. clarify.
+      + i. exploit DOMAIN; eauto.
+        * eapply Genv.genv_symb_range; eauto.
+        * ii. eapply INVCOMPAT in H1; eauto.
+          eapply PUBKEPT; eauto.
+          unfold Genv.public_symbol, proj_sumbool in *. des_ifs.
+      + i. destruct (Genv.block_is_volatile skenv_sys_tgt b1) eqn:VOL1.
+        * dup VOL1. eapply Genv.block_is_volatile_below in VOL1.
+          destruct (classic (mem_inv sm0 b1)).
+          { exfalso. hexploit NDOMAIN; eauto. i. clarify. }
+          { hexploit DOMAIN; eauto. i. clarify. }
+        * destruct (Genv.block_is_volatile skenv_sys_tgt b2) eqn:VOL2; auto.
+          dup VOL2. eapply Genv.block_is_volatile_below in VOL2.
+          exfalso. exploit IMAGE; eauto. i. clarify.
+    - rewrite MEMSRC. eauto.
+    - i. des. eexists (mk _ _ _ _). exists (Retv.mk vres' m2'). ss.
+      esplits; ss; eauto.
+      + rewrite MEMTGT. eauto.
+      + econs; ss; eauto.
+      + econs; ss; eauto.
+        * rewrite MEMSRC in *. eapply Mem.unchanged_on_nextblock; eauto.
+        * eapply Mem.unchanged_on_nextblock; eauto.
+        * rewrite MEMSRC in *. eauto.
+      + econs; ss; eauto.
+        * eapply unchanged_on_invariant; eauto.
+          { ii. eapply INVRANGE; eauto. apply 0. }
+          { eapply Mem.unchanged_on_implies; eauto.
+            i. rewrite MEMSRC. eapply INVRANGE; eauto. }
+        * ii. exploit INVRANGE; eauto. i. des. split.
+          { ii. eapply H6; eauto.
+            - instantiate (1:=delta). instantiate (1:=b0).
+              destruct (inj sm0 b0) as [[blk0 delta0]|] eqn:DELTA.
+              + eapply H4 in DELTA. clarify.
+              + exfalso. exploit H5; eauto. i. des. clarify.
+            - rewrite MEMSRC in *. eapply external_call_max_perm; eauto.
+              destruct (inj sm0 b0) as [[blk0 delta0]|] eqn:DELTA.
+              + dup DELTA. eapply H4 in DELTA. clarify.
+                eapply Mem.valid_block_inject_1; eauto.
+              + exfalso. exploit H5; eauto. i. des. clarify. }
+          { eapply Plt_Ple_trans; eauto.
+            eapply Mem.unchanged_on_nextblock; eauto. }
+  Qed.
 
 End SIMSYMBINV.
